

MATH 2101 Linear Algebra I–Matrix Algebra

What to study in Linear Algebra?

- ① **Systems of linear equations:** One consider the solution (x_1, \dots, x_n) for

$$x_1 + 2x_2 + \dots + nx_n = 0$$

For example, $(2, -1, 0, \dots, 0)$ and $(0, 3, -2, 0, \dots, 0)$ are solutions for the equation. How do you obtain more solutions form these two?

- ② One central object in linear algebra is **matrices**.

This course will emphasis on both *conceptual* and *practical* sides of linear algebras.

Matrix

Definition

- ① A $n \times m$ matrix is a rectangular array of the form:

$$\begin{pmatrix} a_{11} & a_{12} & \cdots & a_{1m} \\ a_{21} & a_{22} & \cdots & a_{2m} \\ \vdots & \vdots & & \vdots \\ a_{n1} & a_{n2} & \cdots & a_{nm} \end{pmatrix}$$

where a_{ij} are in \mathbb{R} .

- ② We shall also sometimes simply write (a_{ij}) to represent an arbitrary matrix, whose (i,j) -**entry** is a_{ij} .
 ③ For a matrix A , we write A_{ij} to be the (i,j) entry of A .

- ④ The i' -**th row** of (a_{ij}) is the $1 \times m$ matrix $(a_{i'1} \quad a_{i'2} \quad \cdots \quad a_{i'm})$

- ⑤ The j' -**th column** of (a_{ij}) is the $n \times 1$ matrix $\begin{pmatrix} a_{1j'} \\ a_{2j'} \\ \vdots \\ a_{nj'} \end{pmatrix}$.

Example

Let $A = \begin{pmatrix} 2 & 4 & 1 \\ 0 & 7 & 9 \end{pmatrix}$. Then

- $A_{13} = 1$
- The 2nd column of A is $\begin{pmatrix} 4 \\ 7 \end{pmatrix}$
- The 1st row of A is $(2 \ 4 \ 1)$.

Vectors

We shall denote \mathbb{R}^n to be the set of n -tuples of numbers in \mathbb{R} . Elements in \mathbb{R}^n can be written as **column vectors**:

$$\begin{pmatrix} a_1 \\ \vdots \\ a_n \end{pmatrix}$$

and is also sometimes written as row vectors (a_1, \dots, a_n) .

- We could add two vectors: e.g.

$$(2, 3) + (4, -1) = (6, 2)$$

- We could also do the scalar multiplication on vectors: e.g.

$$3 \cdot (3, 2) = (9, 6)$$

Adding two matrices

Addition of two $n \times m$ matrices:

$$\begin{pmatrix} a_{11} & a_{12} & \cdots & a_{1m} \\ a_{21} & a_{22} & \cdots & a_{2m} \\ \vdots & \vdots & & \vdots \\ a_{n1} & a_{n2} & \cdots & a_{nm} \end{pmatrix} + \begin{pmatrix} b_{11} & b_{12} & \cdots & b_{1m} \\ b_{21} & b_{22} & \cdots & b_{2m} \\ \vdots & \vdots & & \vdots \\ b_{n1} & b_{n2} & \cdots & b_{nm} \end{pmatrix} = \begin{pmatrix} a_{11} + b_{11} & a_{12} + b_{12} & \cdots & a_{1m} + b_{1m} \\ a_{21} + b_{21} & a_{22} + b_{22} & \cdots & a_{2m} + b_{2m} \\ \vdots & \vdots & & \vdots \\ a_{n1} + b_{n1} & a_{n2} + b_{n2} & \cdots & a_{nm} + b_{nm} \end{pmatrix}$$

Example

$$\begin{pmatrix} 1 & 2 & 4 \\ -1 & 7 & 2 \end{pmatrix} + \begin{pmatrix} -1 & 3 & 2 \\ 1 & 3 & 8 \end{pmatrix} = \begin{pmatrix} 0 & 5 & 6 \\ 0 & 10 & 10 \end{pmatrix}.$$

Scalar multiplication

Scalar multiplication on a $n \times m$ matrix: for a scalar $c \in \mathbb{R}$,

$$c \begin{pmatrix} a_{11} & a_{12} & \dots & a_{1m} \\ a_{21} & a_{22} & \dots & a_{2m} \\ \vdots & \vdots & & \vdots \\ a_{n1} & a_{n2} & \dots & a_{nm} \end{pmatrix} = \begin{pmatrix} ca_{11} & ca_{12} & \dots & ca_{1m} \\ ca_{21} & ca_{22} & \dots & ca_{2m} \\ \vdots & \vdots & & \vdots \\ ca_{n1} & ca_{n2} & \dots & ca_{nm} \end{pmatrix}$$

Matrix multiplication

Matrix multiplication: Let $A = (a_{ij})$ be a $n \times m$ matrix and let $B = (b_{ij})$ be a $m \times p$ matrix. We define the multiplication AB as:

$$(AB)_{ij} = \sum_{x=1}^m a_{ix} b_{xj}$$

Thus matrix multiplication is not even defined if $n \neq m$.

Example

$$(1 \quad 2 \quad 3) \begin{pmatrix} 4 & 3 \\ 0 & 1 \\ 9 & 2 \end{pmatrix} = (1(4) + 2(0) + 3(9) \quad 1(3) + 2(1) + 3(2)) = (31 \quad 11)$$

remark

Where does the matrix multiplication come from? (Or why define in such way?) Consider $A = \begin{pmatrix} 2 & 3 & 0 \\ 1 & 0 & -1 \end{pmatrix}$ and $B = \begin{pmatrix} 3 & 4 \\ 1 & 2 \end{pmatrix}$. Define a map

$T_A : \mathbb{R}^3 \rightarrow \mathbb{R}^2$ by

$$T_A(v) = Av \quad (v \text{ is a column vector in } \mathbb{R}^3),$$

$T_B : \mathbb{R}^2 \rightarrow \mathbb{R}^2$ by

$$T_B(w) = Bw$$

Exercise: Show that

$$(T_B \circ T_A)(v) = (BA)v$$

Property of matrix multiplication I: associativity

Theorem

(Associativity) *The matrix multiplication is an associative operation, meaning that: Let A be a $n \times m$ matrix. Let B be a $m \times p$ matrix. Let C be a $p \times q$ matrix. Then*

$$A(BC) = (AB)C.$$

Proof.

Write $A = (a_{ij})$, $B = (b_{jk})$ and $C = (c_{kl})$. Then

$$(AB)_{ij} = \sum_{x=1}^m a_{ix}b_{xj}, \quad ((AB)C)_{il} = \sum_{y=1}^p (AB)_{iy}C_{yl} = \sum_{y=1}^p \sum_{x=1}^m a_{ix}b_{xy}c_{yl}$$

On the other hand,

$$(BC)_{kl} = \sum_{y=1}^p b_{ky}c_{yl}, \quad A(BC)_{il} = \sum_{x=1}^m a_{ix}(BC)_{xl} = \sum_{x=1}^m \sum_{y=1}^p a_{ix}b_{xy}c_{yl}.$$

Property of matrix multiplication II: distributive

Another property is the distributive:

Theorem

For a $n \times m$ matrix A and $m \times p$ matrices B, C , we have:

$$A(B + C) = AB + AC.$$

Exercise

Verify that $A(B + C) = AB + AC$ by using definitions.

Non-commutativity

For a $n \times m$ matrix A and a $m \times p$ matrix B , we *do not* have $AB = BA$ in general.

Example

Let $A = \begin{pmatrix} 1 & a \\ 0 & 1 \end{pmatrix}$ and $B = \begin{pmatrix} 1 & 0 \\ b & 1 \end{pmatrix}$. Then

$$AB = \begin{pmatrix} 1 + ab & a \\ b & 1 \end{pmatrix}$$

and

$$BA = \begin{pmatrix} 1 & a \\ b & 1 + ab \end{pmatrix}.$$

Identity matrix

The identity matrix I_n is defined as:

$$I_n = \begin{pmatrix} 1 & 0 & \dots & 0 \\ 0 & 1 & \dots & \vdots \\ \vdots & \dots & \dots & \vdots \\ 0 & 0 & \dots & 1 \end{pmatrix},$$

that is

$$(I_n)_{ij} = \begin{cases} 1 & i = j \\ 0 & i \neq j \end{cases}$$

Multiplication with an identity matrix

Theorem

Let A be an $n \times m$ matrix. Then

- ① $I_n A = A$; and
- ② $A I_m = A$.

Proof.

Exercise. □

Exercise

An $n \times n$ matrix A is said to be *diagonal* if for any i, j with $i \neq j$, $A_{ij} = 0$. For example, $\begin{pmatrix} 1 & 0 \\ 0 & 7 \end{pmatrix}$ is diagonal but $\begin{pmatrix} 1 & 3 \\ 0 & 2 \end{pmatrix}$ is not diagonal. Let D be a $n \times n$ diagonal matrix and let E be a $m \times m$ diagonal matrix. Let A be a $n \times m$ matrix.

- ① For a diagonal $n \times n$ matrix D , describe the matrix multiplication DA ;
- ② For a diagonal $m \times m$ matrix E , describe the matrix multiplication AE .

Zero matrices

The $n \times m$ matrix is called the **zero matrix** $0_{n \times m}$ (or sometimes simply 0) if all its entries are zero. The main properties of the zero matrix is the following:

Theorem

Let A be an $n \times m$ matrix. Then

- ① $0_{p \times n}A = 0_{p \times m}$; and
- ② $A0_{m \times q} = 0_{n \times q}$; and
- ③ $A + 0 = A$.

Proof.

Exercise. □

Transpose of a matrix

Definition

The *transpose* of an $n \times m$ matrix A is the $m \times n$ matrix obtained from interchanging rows and columns i.e.

$$(A^T)_{ij} = A_{ji}$$

Example

① Let $A = \begin{pmatrix} 3 & 5 & 0 \end{pmatrix}$. Then

$$A^T = \begin{pmatrix} 3 \\ 5 \\ 0 \end{pmatrix}.$$

② Let $B = \begin{pmatrix} 4 & 1 \\ 0 & 3 \end{pmatrix}$. Then $B^T = \begin{pmatrix} 4 & 0 \\ 1 & 3 \end{pmatrix}$.

Properties of the transpose

Theorem

- ① For $n \times m$ -matrices A and B , $(A + B)^T = A^T + B^T$.
- ② For an $n \times m$ -matrix A and a $m \times p$ -matrix B , $(AB)^T = B^T A^T$.
- ③ For a $n \times m$ -matrix A and a scalar c , $(cA)^T = cA^T$.

Example

Let $A = \begin{pmatrix} 1 & 2 \\ 2 & -1 \end{pmatrix}$ and let $B = \begin{pmatrix} -3 \\ 2 \end{pmatrix}$. Then

$$AB = \begin{pmatrix} 1 & 2 \\ 2 & -1 \end{pmatrix} \begin{pmatrix} -3 \\ 2 \end{pmatrix} = \begin{pmatrix} 1 \\ -8 \end{pmatrix},$$

and so

$$(AB)^T = (1 \quad -8), \quad B^T A^T = (-3 \quad 2) \begin{pmatrix} 1 & 3 \\ 2 & -1 \end{pmatrix} = (1 \quad -8).$$

Where does the transpose come from?

Theorem

For $x = (x_1, \dots, x_n) \in \mathbb{R}^n$ and $y = (y_1, \dots, y_n) \in \mathbb{R}^n$, define

$$\langle x, y \rangle = x_1 y_1 + \dots + x_n y_n.$$

Then, for any $n \times n$ matrix A , $\langle xA, y \rangle = \langle x, yA^T \rangle$.

Proof.

One can write $\langle x, y \rangle$ as:

$$\langle x, y \rangle = xy^T.$$

Hence,

$$\langle xA, y \rangle = xAy^T$$



Doing transpose twice

Theorem

Let A be an $n \times m$ matrix. Then $(A^T)^T = A$.

Proof.

$$((A^T)^T)_{ij} = (A^T)_{ji} = A_{ij}.$$

